Overhaul obj? (Part 2)

src/ReactorModel/Objects/Reactor/Indexable.lean
@@ -11,21 +11,10 @@ def UniqueIDs [ReactorType α] (rtr : α) : Prop :=
 class Indexable (α) extends ReactorType α where
   unique_ids : ∀ {rtr : α}, UniqueIDs rtr
 
-namespace Indexable
-
-variable [Indexable α]
-
-def obj? (rtr : α) (cpt : Component) : cpt.idType ⇀ cpt.type α :=
+def Indexable.obj? [Indexable α] (rtr : α) (cpt : Component) : cpt.idType ⇀ cpt.type α :=
   fun i => if h : ∃ o, Object rtr cpt i o then h.choose else none
 
-notation (priority := 1001) rtr "[" cpt "]" => obj? rtr cpt
-notation rtr "[" cpt "][" i "]"             => obj? rtr cpt i 
+notation (priority := 1001) rtr "[" cpt "]" => Indexable.obj? rtr cpt
+notation rtr "[" cpt "][" i "]"             => Indexable.obj? rtr cpt i 
 
-def con? (rtr : α) (cpt : Component) : ID ⇀ Container α := 
-  fun i => if s : Nonempty (StrictMember cpt i rtr) then s.some.container else none
-
-notation rtr "[" cpt "]&"        => con? rtr cpt
-notation rtr "[" cpt "][" i "]&" => con? rtr cpt i
-
-end Indexable
 end ReactorType
