src/ReactorModel/Determinism/Dependency.lean
@@ -2,121 +2,45 @@ import ReactorModel.Execution
 
 open Classical ReactorType Indexable
 
--- TODO: Move this into `Objects.Reactor.Theorems`.
-namespace ReactorType
-namespace Wellformed
-
-variable [Indexable α] {rtr : α} (wf : Wellformed rtr)
-
-theorem shared_dep_local 
-    (h₁ : rtr[.rcn][i₁] = some rcn₁) (h₂ : rtr[.rcn][i₂] = some rcn₂) (hd₁ : ⟨cpt, j⟩ ∈ rcn₁.deps k)
-    (hd₂ : ⟨cpt, j⟩ ∈ rcn₂.deps k) : rtr[.rcn][i₁]& = rtr[.rcn][i₂]& := by
-  by_cases hi : i₁ = i₂
-  case pos => simp_all
-  case neg =>
-    apply con?_eq_ext h₁ h₂
-    intro _ _ hc₁ hc₂ hr₁ hr₂
-    have hv₁ := wf.valid_deps hc₁ hr₁ hd₁
-    have hv₂ := wf.valid_deps hc₂ hr₂ hd₂
-    cases k <;> cases cpt <;> try cases ‹Kind› 
-    case out.prt.in => exact absurd hd₂ $ wf.unique_inputs h₁ h₂ hi hd₁
-    case in.prt.out =>
-      cases hk₁ : rcn₁.kind <;> cases hk₂ : rcn₂.kind <;> cases hk₁ ▸ hv₁ <;> cases hk₂ ▸ hv₂
-      case _ hn₁ hj₁ _ _ hn₂ hj₂ =>
-        have hc₁' := obj?_rtr_and_cpt?_to_obj? hc₁ (cpt := .rtr) hn₁
-        have hc₂' := obj?_rtr_and_cpt?_to_obj? hc₂ (cpt := .rtr) hn₂
-        have hj := mem_cpt?_rtr_eq hc₁' hc₂' (cpt := .prt .out) hj₁ hj₂
-        have hn₁ := Partial.mem_iff.mpr ⟨_, hn₁⟩ 
-        have hn₂ := Partial.mem_iff.mpr ⟨_, hn₂⟩ 
-        injection hj with hj
-        exact mem_cpt?_rtr_eq hc₁ hc₂ (cpt := .rtr) hn₁ (hj ▸ hn₂)
-    all_goals 
-      cases hk₁ : rcn₁.kind <;> cases hk₂ : rcn₂.kind <;> cases hk₁ ▸ hv₁ <;> cases hk₂ ▸ hv₂
-      all_goals first 
-        | exact mem_cpt?_rtr_eq hc₁ hc₂ (cpt := .stv) ‹_› ‹_› 
-        | exact mem_cpt?_rtr_eq hc₁ hc₂ (cpt := .act) ‹_› ‹_›
-        | exact mem_cpt?_rtr_eq hc₁ hc₂ (cpt := .prt .out) ‹_› ‹_›
-        | exact mem_cpt?_rtr_eq hc₁ hc₂ (cpt := .prt .in) ‹_› ‹_›
-
-theorem shared_state_local
-    (h₁ : rtr[.rcn][i₁] = some rcn₁) (h₂ : rtr[.rcn][i₂] = some rcn₂) 
-    (hd₁ : ⟨.stv, j⟩ ∈ rcn₁.deps k₁) (hd₂ : ⟨.stv, j⟩ ∈ rcn₂.deps k₂) : 
-    rtr[.rcn][i₁]& = rtr[.rcn][i₂]& := by
-  apply con?_eq_ext h₁ h₂
-  intro _ _ hc₁ hc₂ hr₁ hr₂
-  have hv₁ := wf.valid_deps hc₁ hr₁ hd₁
-  have hv₂ := wf.valid_deps hc₂ hr₂ hd₂
-  cases hk₁ : rcn₁.kind <;> cases hk₂ : rcn₂.kind <;> cases hk₁ ▸ hv₁ <;> cases hk₂ ▸ hv₂
-  all_goals exact mem_cpt?_rtr_eq hc₁ hc₂ (cpt := .stv) ‹_› ‹_› 
-
-theorem hazards_prio' 
-    (h₁ : rtr[.rcn][i₁] = some rcn₁) (h₂ : rtr[.rcn][i₂] = some rcn₂) (hn : i₁ ≠ i₂)
-    (hc : rtr[.rcn][i₁]& = rtr[.rcn][i₂]&) (hd₁ : ⟨.stv, j⟩ ∈ rcn₁.deps k₁) 
-    (hd₂ : ⟨.stv, j⟩ ∈ rcn₂.deps k₂) (hk : k₁ = .out ∨ k₂ = .out) :
-    rcn₁.prio < rcn₂.prio ∨ rcn₂.prio < rcn₁.prio :=
-  have ⟨_, _, hc, hr₁, hr₂⟩ := obj?_con?_eq h₁ h₂ hc 
-  wf.hazards_prio hc hr₁ hr₂ hn hd₁ hd₂ hk
-
-theorem overlap_prio' 
-    (h₁ : rtr[.rcn][i₁] = some rcn₁) (h₂ : rtr[.rcn][i₂] = some rcn₂) (hn : i₁ ≠ i₂)
-    (hc : rtr[.rcn][i₁]& = rtr[.rcn][i₂]&) (hd₁ : d ∈ rcn₁.deps .out) (hd₂ : d ∈ rcn₂.deps .out) :
-    rcn₁.prio < rcn₂.prio ∨ rcn₂.prio < rcn₁.prio :=
-  have ⟨_, _, hc, hr₁, hr₂⟩ := obj?_con?_eq h₁ h₂ hc 
-  wf.overlap_prio hc hr₁ hr₂ hn hd₁ hd₂
-
-end Wellformed
-end ReactorType
-
 namespace Dependency
-
-theorem prio' [Indexable α] {rtr : α}
-    (h₁ : rtr[.rcn][i₁] = some rcn₁) (h₂ : rtr[.rcn][i₂] = some rcn₂) 
-    (hc : rtr[.rcn][i₁]& = rtr[.rcn][i₂]&) (hm : rcn₁.Mutates ↔ rcn₂.Mutates) 
-    (hp : rcn₁.prio > rcn₂.prio) : i₁ <[rtr] i₂ :=
-  have ⟨_, _, hc, hr₁, hr₂⟩ := obj?_con?_eq h₁ h₂ hc 
-  Dependency.prio hc hr₁ hr₂ hm hp
-
-theorem mutNorm' [Indexable α] {rtr : α}
-    (h₁ : rtr[.rcn][iₘ] = some m) (h₂ : rtr[.rcn][iₙ] = some n) (hm : m.Mutates) (hn : n.Normal)
-    (hc : rtr[.rcn][iₘ]& = rtr[.rcn][iₙ]&) : iₘ <[rtr] iₙ :=
-  have ⟨_, _, hc, hr₁, hr₂⟩ := obj?_con?_eq h₁ h₂ hc 
-  Dependency.mutNorm hc hr₁ hr₂ hm hn
 
 variable [Proper α] {rtr : α}
 
-theorem same_con_shared_out_dep
-    (h₁ : rtr[.rcn][i₁] = some rcn₁) (h₂ : rtr[.rcn][i₂] = some rcn₂)
-    (hc : rtr[.rcn][i₁]& = rtr[.rcn][i₂]&) (hn : i₁ ≠ i₂) (hd₁ : ⟨cpt, i⟩ ∈ Reaction.deps rcn₁ .out) 
-    (hd₂ : ⟨cpt, i⟩ ∈ Reaction.deps rcn₂ .out) : (i₁ <[rtr] i₂) ∨ (i₂ <[rtr] i₁) := by
+theorem same_con_needOrderedPriority
+    (hc : rtr[.rtr][c] = some con) (h₁ : get? con .rcn i₁ = some rcn₁) 
+    (h₂ : get? con .rcn i₂ = some rcn₂) (hn : i₁ ≠ i₂) 
+    (hp : Wellformed.NeedOrderedPriority rcn₁ rcn₂) : (i₁ <[rtr] i₂) ∨ (i₂ <[rtr] i₁) := by
   by_cases hm₁ : rcn₁.Mutates <;> by_cases hm₂ : rcn₂.Mutates
   rotate_left
-  · exact .inl $ Dependency.mutNorm' h₁ h₂ hm₁ (by simp_all [Reaction.Mutates]) hc
-  · exact .inr $ Dependency.mutNorm' h₂ h₁ hm₂ (by simp_all [Reaction.Mutates]) hc.symm
+  · exact .inl $ .mutNorm hc h₁ h₂ hm₁ (by simp_all [Reaction.Mutates])
+  · exact .inr $ .mutNorm hc h₂ h₁ hm₂ (by simp_all [Reaction.Mutates])
   all_goals
-    cases Proper.wellformed rtr |>.overlap_prio' h₁ h₂ hn hc hd₁ hd₂
-    · exact .inr $ Dependency.prio' h₂ h₁ hc.symm (by simp_all) ‹_›
-    · exact .inl $ Dependency.prio' h₁ h₂ hc (by simp_all) ‹_›
+    cases Proper.wellformed rtr |>.ordered_prio hc h₁ h₂ hn hp
+    · exact .inr $ .prio hc h₂ h₁ (by simp_all) ‹_›
+    · exact .inl $ .prio hc h₁ h₂ (by simp_all) ‹_›
+
+theorem hazard 
+    (hc : rtr[.rtr][c] = some con) (h₁ : get? con .rcn i₁ = some rcn₁) 
+    (h₂ : get? con .rcn i₂ = some rcn₂) (hn : i₁ ≠ i₂) (hd₁ : ⟨.stv, i⟩ ∈ Reaction.deps rcn₁ k₁) 
+    (hd₂ : ⟨.stv, i⟩ ∈ Reaction.deps rcn₂ k₂) (hk : k₁ = .out ∨ k₂ = .out) : 
+    (i₁ <[rtr] i₂) ∨ (i₂ <[rtr] i₁) := 
+  same_con_needOrderedPriority hc h₁ h₂ hn (.hazard hd₁ hd₂ hk)
+
+theorem same_con_shared_out_dep
+    (hc : rtr[.rtr][c] = some con) (h₁ : get? con .rcn i₁ = some rcn₁) 
+    (h₂ : get? con .rcn i₂ = some rcn₂) (hn : i₁ ≠ i₂) (hd₁ : ⟨cpt, i⟩ ∈ Reaction.deps rcn₁ .out) 
+    (hd₂ : ⟨cpt, i⟩ ∈ Reaction.deps rcn₂ .out) : (i₁ <[rtr] i₂) ∨ (i₂ <[rtr] i₁) :=
+  same_con_needOrderedPriority hc h₁ h₂ hn (.overlap hd₁ hd₂)
 
 theorem shared_out_dep
     (h₁ : rtr[.rcn][i₁] = some rcn₁) (h₂ : rtr[.rcn][i₂] = some rcn₂) (hn : i₁ ≠ i₂)
     (hd₁ : ⟨cpt, i⟩ ∈ Reaction.deps rcn₁ .out) (hd₂ : ⟨cpt, i⟩ ∈ Reaction.deps rcn₂ .out) :
     (i₁ <[rtr] i₂) ∨ (i₂ <[rtr] i₁) := by  
-  have hc := Proper.wellformed rtr |>.shared_dep_local h₁ h₂ hd₁ hd₂
-  exact same_con_shared_out_dep h₁ h₂ hc hn hd₁ hd₂
-
-theorem hazard 
-    (h₁ : rtr[.rcn][i₁] = some rcn₁) (h₂ : rtr[.rcn][i₂] = some rcn₂) (hn : i₁ ≠ i₂)
-    (hc : rtr[.rcn][i₁]& = rtr[.rcn][i₂]&) (hd₁ : ⟨.stv, i⟩ ∈ Reaction.deps rcn₁ k₁) 
-    (hd₂ : ⟨.stv, i⟩ ∈ Reaction.deps rcn₂ k₂) (hk : k₁ = .out ∨ k₂ = .out) : 
-    (i₁ <[rtr] i₂) ∨ (i₂ <[rtr] i₁) := by  
-  by_cases hm₁ : rcn₁.Mutates <;> by_cases hm₂ : rcn₂.Mutates
-  rotate_left
-  · exact .inl $ Dependency.mutNorm' ‹_› ‹_› hm₁ (by simp_all [Reaction.Mutates]) hc
-  · exact .inr $ Dependency.mutNorm' ‹_› ‹_› hm₂ (by simp_all [Reaction.Mutates]) hc.symm
-  all_goals
-    cases Proper.wellformed rtr |>.hazards_prio' h₁ h₂ hn hc hd₁ hd₂ hk
-    · exact .inr $ Dependency.prio' h₂ h₁ hc.symm (by simp_all) ‹_›
-    · exact .inl $ Dependency.prio' h₁ h₂ hc (by simp_all) ‹_›
+  have ⟨_, _, hc₁, hr₁⟩ := obj?_some_split h₁
+  have ⟨_, _, hc₂, hr₂⟩ := obj?_some_split h₂
+  have hc := Proper.wellformed rtr |>.shared_dep_local hc₁ hc₂ hr₁ hr₂ hd₁ hd₂
+  injection hc₂ ▸ hc ▸ hc₁ with hc
+  exact same_con_shared_out_dep hc₁ hr₁ (hc ▸ hr₂) hn hd₁ hd₂
 
 end Dependency
 
@@ -124,16 +48,20 @@ end Dependency
 abbrev NotDependent [Indexable α] (rtr : α) (rcn₁ rcn₂ : ID) : Prop :=
   ¬(rcn₁ <[rtr] rcn₂)
 
+namespace NotDependent
+
 notation:50 rcn₁ " ≮[" rtr "] " rcn₂ => NotDependent rtr rcn₁ rcn₂
 
-theorem NotDependent.equiv [Indexable α] {rtr₁ rtr₂ : α} (h : i₁ ≮[rtr₁] i₂) (e : rtr₁ ≈ rtr₂) : 
+theorem equiv [Indexable α] {rtr₁ rtr₂ : α} (h : i₁ ≮[rtr₁] i₂) (e : rtr₁ ≈ rtr₂) : 
     i₁ ≮[rtr₂] i₂ :=
   (h $ ·.equiv e)
 
-theorem NotDependent.deps_disjoint [Indexable α] {rtr : α} {d} (hi : i₁ ≮[rtr] i₂) 
+theorem deps_disjoint [Indexable α] {rtr : α} {d} (hi : i₁ ≮[rtr] i₂) 
     (h₁ : rtr[.rcn][i₁] = some rcn₁) (h₂ : rtr[.rcn][i₂] = some rcn₂) (h : d ∈ rcn₁.deps .out) 
     (hs : d.cpt ≠ .stv) : d ∉ rcn₂.deps .in :=
-  byContradiction fun hd => hi $ Dependency.depOverlap h₁ h₂ h (not_not.mp hd) hs
+  byContradiction fun hd => hi $ .depOverlap h₁ h₂ h (not_not.mp hd) hs
+
+end NotDependent
 
 structure Independent [Indexable α] (rtr : α) (rcn₁ rcn₂ : ID) : Prop where
   not_eq : rcn₁ ≠ rcn₂  
@@ -161,8 +89,12 @@ theorem no_shared_state_deps [Proper α] {rtr : α}
   have hd₁ := rcn₁.target_mem_deps hs
   simp [Change.Normal.target] at hd₁
   by_contra hd₂
-  have hc := Proper.wellformed rtr |>.shared_state_local h₁ h₂ hd₁ hd₂
-  cases Dependency.hazard h₁ h₂ hi.not_eq hc hd₁ hd₂ (.inl rfl) <;> simp [hi.left, hi.right] at *
+  have ⟨_, _, hc₁, hr₁⟩ := obj?_some_split h₁
+  have ⟨_, _, hc₂, hr₂⟩ := obj?_some_split h₂
+  have hc := Proper.wellformed rtr |>.shared_state_local hc₁ hc₂ hr₁ hr₂ hd₁ hd₂
+  injection hc₂ ▸ hc ▸ hc₁ with hc
+  cases Dependency.hazard hc₁ hr₁ (hc ▸ hr₂) hi.not_eq hd₁ hd₂ (.inl rfl) 
+  all_goals simp [hi.left, hi.right] at *
 
 end Independent
 
